new bookperm from book

acl2/.#ssy1.lisp
@@ -1,1 +1,0 @@
-syshen@syshen-ThinkPad-X201.10255:1446686129
