acl2/ssy1.lisp
@@ -1,3 +1,35 @@
+(defun insert (x y)
+  (cond ((endp y) (list x))
+        ((<= x (car y)) (cons x y))
+        (t (cons (car y) (insert x (cdr y))))
+        )
+  )
+
+(defun insert-sort (x)
+  (cond ((endp x) nil)
+        (t (insert (car x) 
+		   (insert-sort (cdr x))))
+        )
+)
+
+(defun is-sorted (x)
+  (cond ((endp x) t)
+        ((endp (cdr x)) t)
+        (t (and (<= (car x) (car (cdr x)) ) 
+                (is-sorted (cdr x)) ) 
+           ))
+  )
+
+(defthm is-sorted-insert 
+  (implies (is-sorted y)
+           (is-sorted (insert x y))
+           )
+  )
+
+(defthm is-sorted-insert-sort 
+  (is-sorted (insert-sort x))
+  )
+
 (defun ismem (x y)
   (cond  ((endp y) nil)
          ((equal x (car y)) t)
@@ -22,19 +54,93 @@
   (perm x x)
 )
 
-(defun insert (x y)
-  (cond ((endp y) (list x))
-        ((< x (car y)) (cons x y))
-        (t (cons (car y) (insert x (cdr y))))
-        )
+
+(defthm insert-sort-is-sort
+  (is-sorted (insert-sort x))
   )
 
-(defun insert-sort (x)
-  (cond ((endp x) nil)
-        (t (insert (car x) 
-		   (insert-sort (cdr x))))
-        )
-)
+(defthm insert-sort-sub-is-sorted
+  (implies (is-sorted x)
+           (is-sorted (cdr x)))
+  )
+
+
+;; not proved yet
+(defthm cons-x-nil
+  (implies (not (consp y))
+           (equal (cons x y) x)
+           )
+  )
+
+
+(defthm one-car-equal-x
+  (IMPLIES (AND (CONSP X) (NOT (CONSP (CDR X))))
+           (EQUAL (LIST (CAR X)) X)
+           )
+  )
+
+
+
+(defthm insert-car-cdr-equal-x
+  (implies (and (is-sorted x)
+                (consp x))
+           (equal (insert (car x) (cdr x))
+                  x)
+           )
+  )
+
+
+
+
+
+
+
+
+(defthm sorted-insert-car-cdr-not-change
+  (implies (is-sorted x)
+           (equal (insert (car x)
+                          (cdr x)
+                          )
+                  x))
+  )
+
+
+(defthm sorted-equal
+  (implies (is-sorted x)
+           (equal (insert-sort x) x))
+  )
+
+(defthm perm-sort-norm
+  (implies (and (is-sorted x)
+                (perm x y))
+           (perm x (insert-sort y))
+           )
+  )
+
+(defthm perm-insert-sort
+  (implies (perm x y)
+           (equal (insert-sort x) 
+                  (insert-sort y)))
+  )
+
+(defthm perm-cons
+  (implies (perm x y)
+           (perm (insert a x) (cons a y)))
+  )
+
+
+
+
+
+(defthm insert-sort-is-perm
+  (perm (insert-sort x) x)
+  )
+
+
+
+
+
+
 
 
 (defthm ismem-insert
