acl2/bookperm.lisp
@@ -1,0 +1,74 @@
+(defun insert (a x)
+  (cond ((atom x) (list a))
+        ((<= a (car x)) (cons a x))
+        (t (cons (car x) (insert a (cdr x))))))
+(defun insertion-sort (x)
+  (cond ((atom x) nil)
+        (t (insert (car x) (insertion-sort (cdr x))))))
+(defun orderedp (x)
+  (cond ((atom (cdr x)) t)
+        (t (and (<= (car x) (cadr x))
+                (orderedp (cdr x))))))
+
+(defthm insertion-sort-is-ordered
+  (orderedp (insertion-sort x)))
+
+
+
+(defun in (a b)
+  (cond ((atom b) nil)
+        ((equal a (car b)) t)
+        (t (in a (cdr b)))))
+(defun del (a x)
+  (cond ((atom x) nil)
+        ((equal a (car x)) (cdr x))
+        (t (cons (car x) (del a (cdr x))))))
+
+(defun perm (x y)
+  (cond ((atom x) (atom y))
+        (t (and (in (car x) y)
+                (perm (cdr x) (del (car x) y))))))
+
+
+(defthm insertion-sort-is-perm
+  (perm (insertion-sort x) x))
+
+
+(defthm insert-perm-cons
+  (implies (perm x y)
+           (perm (insert a x) (cons a y))))
+
+
+(defthm insert-ordered
+  (implies (orderedp x)
+           (orderedp (insert a x))))
+
+(defthm perm-reflex
+  (perm x x))
+
+
+
+
+
+
+; define a normal form
+(defthm orderedp-x-sort-not-change
+  (implies (and (orderedp x)
+                (consp x))
+           (equal (insertion-sort x) x) 
+           ))
+
+
+
+
+
+
+
+
+
+
+
+
+
+(defthm perm-sym
+  (implies (perm x y) (perm y x)))
